Environment refactor finished
Only not fixed: BigStep/EvalExamples/inf_diverges

News:
BigStep/SemanticsProofs.
+ append_vars_to_env_step
+ append_vars_to_env_single
+ get_value_here_new
+ get_value_there_new

src/BigStep/Environment.v
@@ -24,30 +24,27 @@ match env with
 end.
 
 (** Insert *)
+(* DEPRICATED *)
 Definition insert_value (env : Environment) (key : (Var + FunctionIdentifier)) 
    (value : Value) : Environment :=
 (key, value) :: env.
-(* match env with
-  | [] => [(key, value)]
-  | (k,v)::xs => if var_funid_eqb k key then (key,value)::xs else (k,v)::(insert_value xs key value)
-end. *)
+
+(** Zip **)
+Fixpoint zip {A B : Type} (al : list A) (bl : list B) : list (A * B) :=
+match al, bl with
+| a :: al', b :: bl' => (a, b) :: zip al' bl'
+| _, _ => []
+end.
 
 (** Add additional bindings *)
 (** We used here: when binding, variables must be unique *)
-Fixpoint add_bindings (bindings : list (Var * Value)) (env : Environment) : Environment :=
-match bindings with
-| [] => env
-| (v, e)::xs => add_bindings xs (insert_value env (inl v) e)
-end.
+Definition add_bindings (bindings : list (Var * Value)) (env : Environment) : Environment :=
+map (fun '(var, val) => (inl var, val)) bindings ++ env.
 
 (** Add bindings with two lists *)
-Fixpoint append_vars_to_env (vl : list Var) (el : list Value) (d : Environment) 
+Definition append_vars_to_env (vl : list Var) (el : list Value) (d : Environment) 
    : Environment :=
-match vl, el with
-| [], [] => d
-| v::vs, e::es => append_vars_to_env vs es (insert_value d (inl v) e)
-| _, _ => []
-end.
+zip (map inl vl) el ++ d.
 
 
 Definition append_try_vars_to_env (vl : list Var) (el : list Value) (d : Environment) 
@@ -60,31 +57,37 @@ end.
 
 Goal append_try_vars_to_env ["X"%string; "Y"%string] [VNil; VNil; VNil] []
 = [(inl "X"%string, VNil); (inl "Y"%string, VNil)].
-Proof. Admitted.
+Proof. reflexivity. Qed.
 
 (** Not Overwriting insert *)
 (** Overwriting does not fit with this recursion *)
-Fixpoint insert_function (id : nat) (v : FunctionIdentifier) (p : list Var) (b : Expression) 
+(* DEPRICATED *)
+Definition insert_function (id : nat) (v : FunctionIdentifier) (p : list Var) (b : Expression) 
    (l : list (nat * FunctionIdentifier * FunctionExpression)) 
     : list (nat * FunctionIdentifier * FunctionExpression) :=
-match l with
-| [] => [(id, v, (p, b))]
-| (id', k, v0)::xs => if funid_eqb k v then (id', k, v0)::xs 
-                                   else (id', k, v0)::(insert_function id v p b xs)
-end.
+(id, v, (p, b)) :: l.
 
 (** Lists represented functions *)
-Fixpoint list_functions (vl : list FunctionIdentifier) (paramss : list (list Var)) 
+(* DEPRICATED *)
+Fixpoint list_functions_old (vl : list FunctionIdentifier) (paramss : list (list Var)) 
       (bodies : list Expression) (last_id : nat) 
       : list (nat * FunctionIdentifier * FunctionExpression) :=
 match vl, paramss, bodies with
-| [], [], [] => []
-| v::vs, varl::ps, e::bs => insert_function last_id v varl e 
-                                 (list_functions vs ps bs (S last_id))
+| v::vs, varl::ps, e::bs => (last_id, v, (varl, e)) :: list_functions_old vs ps bs (S last_id)
 | _, _, _ => []
 end.
 
+(* DEPRICATED *)
+Fixpoint list_functions (last_id : nat)
+      (l : list (FunctionIdentifier * ((list Var) * Expression)))
+      : list (nat * FunctionIdentifier * FunctionExpression) :=
+match l with
+| (fid, (vars, e)) :: l' => (last_id, fid, (vars, e)) :: list_functions (S last_id) l'
+| [] => []
+end.
+
 (** Add functions *)
+(* DEPRICATED *)
 Fixpoint append_funs_to_env_base (vl : list FunctionIdentifier) (paramss : list (list Var)) 
       (bodies : list Expression) (d : Environment) (def : Environment) 
       (deffuns : list (nat * FunctionIdentifier * FunctionExpression)) (last_id : nat) 
@@ -98,14 +101,28 @@ match vl, paramss, bodies with
 | _, _, _ => []
 end.
 
-Definition append_funs_to_env (l : list (FunctionIdentifier * ((list Var) * Expression))) (d : Environment) (last_id : nat) : Environment :=
+(* DEPRICATED *)
+Definition append_funs_to_env_old (l : list (FunctionIdentifier * ((list Var) * Expression))) (d : Environment) (last_id : nat) : Environment :=
 append_funs_to_env_base (fst (split l)) (fst (split (snd (split l)))) (snd (split (snd (split l)))) d d 
-                       (list_functions (fst (split l)) (fst (split (snd (split l)))) (snd (split (snd (split l)))) last_id)
+                       (list_functions_old (fst (split l)) (fst (split (snd (split l)))) (snd (split (snd (split l)))) last_id)
                        last_id
 .
 
+Definition get_env (env : Environment)
+   (ext : list (nat * FunctionIdentifier * FunctionExpression))
+   : Environment :=
+map
+  (fun '(n, fid, (vars, e)) =>
+    ((inr fid), (VClos env ext n vars e)))
+  ext
+++ env.
+
+Definition append_funs_to_env (l : list (FunctionIdentifier * ((list Var) * Expression))) (d : Environment) (last_id : nat) : Environment :=
+get_env d (list_functions last_id l).
+
+
 (** Examples *)
-Goal append_vars_to_env ["A"%string; "A"%string]
+(* Goal append_vars_to_env ["A"%string; "A"%string]
                            [(VEmptyMap); (VEmptyTuple)]
                            [(inl "A"%string, VEmptyMap)]
 = [(inl "A"%string, VTuple [])].
@@ -125,15 +142,16 @@ Goal append_funs_to_env [(("f1"%string,0), ([], ErrorExp)) ;
          [(2, ("f1"%string, 0), ([], ELit (Atom "error")));
          (1, ("f2"%string, 0), ([], ELit (Atom "error")))] 1 [] (ELit (Atom "error")))].
 Proof. Admitted.
-Goal insert_function 2 ("f1"%string, 0) [] ErrorExp (list_functions
+Goal insert_function 2 ("f1"%string, 0) [] ErrorExp (list_functions_old
                               [("f1"%string,0); ("f2"%string,0); ("f1"%string, 0)]
                               [[];[];[]]
                               [ErrorExp; ErrorExp; ErrorExp] 0)
 = [(2, ("f1"%string, 0), ([], ELit (Atom "error")));
        (1, ("f2"%string, 0), ([], ELit (Atom "error")))].
-Proof. reflexivity. Qed.
+Proof. Admitted. *)
 
 (** Environment construction from the extension and the reference *)
+(* DEPRICATED *)
 Fixpoint get_env_base (env def : Environment) 
    (ext defext : list (nat * FunctionIdentifier * FunctionExpression))
    : Environment :=
@@ -142,7 +160,8 @@ match ext with
 | (id, f1, (pl, b))::xs => get_env_base (insert_value env (inr f1) (VClos def defext id pl b)) def xs defext
 end.
 
-Definition get_env (env : Environment) 
+(* DEPRICATED *)
+Definition get_env_old (env : Environment) 
    (ext : list (nat * FunctionIdentifier * FunctionExpression))
    : Environment :=
   get_env_base env env ext ext
