src/BigStep/SemanticsProofs.v
@@ -630,9 +630,42 @@ Proof.
         ** intros.
 Qed.*)
 
+Lemma append_vars_to_env_step :
+  forall var vars val vals env,
+    append_vars_to_env (var :: vars) (val :: vals) env
+  = (inl var, val) :: append_vars_to_env vars vals env.
+Proof.
+  intros.
+  unfold append_vars_to_env.
+  simpl.
+  reflexivity.
+Qed.
+
+Lemma append_vars_to_env_single :
+  forall var val env,
+    append_vars_to_env [var] [val] env
+  = (inl var, val) :: env.
+Proof.
+  intros.
+  unfold append_vars_to_env.
+  simpl.
+  reflexivity.
+Qed.
+
 (** Last append result *)
 Proposition get_value_here (env : Environment) (var : Var + FunctionIdentifier) (val : Value):
 get_value (insert_value env var val) var = Some [val].
+Proof.
+  induction env.
+  * simpl. rewrite var_funid_eqb_refl. reflexivity.
+  * simpl. destruct a. case_eq (var_funid_eqb s var); intro.
+    - simpl. rewrite var_funid_eqb_refl. reflexivity.
+    - (* simpl. rewrite var_funid_eqb_sym, H. assumption. *)
+      simpl. rewrite var_funid_eqb_refl. reflexivity.
+Qed.
+
+Proposition get_value_here_new (env : Environment) (var : Var + FunctionIdentifier) (val : Value):
+get_value ((var, val) :: env) var = Some [val].
 Proof.
   induction env.
   * simpl. rewrite var_funid_eqb_refl. reflexivity.
@@ -647,6 +680,25 @@ Proposition get_value_there (env : Environment) (var var' : Var + FunctionIdenti
      (val : Value):
 var <> var' ->
 get_value (insert_value env var val) var' = get_value env var'.
+Proof.
+  intro. induction env.
+  * simpl. apply var_funid_eqb_neq in H. rewrite var_funid_eqb_sym in H. rewrite H. reflexivity.
+  * simpl. destruct a. case_eq (var_funid_eqb s var); intro.
+    - apply var_funid_eqb_eq in H0. assert (var <> var'). auto. rewrite <- H0 in H.
+      apply var_funid_eqb_neq in H. rewrite var_funid_eqb_sym in H. rewrite H. simpl. apply var_funid_eqb_neq in H1.
+      rewrite var_funid_eqb_sym in H1. rewrite H1. reflexivity.
+    - simpl. case_eq (var_funid_eqb var' s); intros.
+      + (* reflexivity. *)
+        rewrite var_funid_eqb_neq in H0. rewrite var_funid_eqb_eq in H1.
+        rewrite <- H1 in H0. rewrite <- var_funid_eqb_neq in H0.
+        rewrite H0. reflexivity.
+      + apply IHenv.
+Qed.
+
+Proposition get_value_there_new (env : Environment) (var var' : Var + FunctionIdentifier) 
+     (val : Value):
+var <> var' ->
+get_value ((var, val) :: env) var' = get_value env var'.
 Proof.
   intro. induction env.
   * simpl. apply var_funid_eqb_neq in H. rewrite var_funid_eqb_sym in H. rewrite H. reflexivity.
